theories/lang/lifting.v
@@ -255,8 +255,8 @@ Lemma wp_cas_fail vl1 vl2 vd vo ve z1 z2 Φ l1 l2 it q E:
   val_to_loc vl2 = Some l2 →
   l1 `has_layout_loc` it_layout it →
   l2 `has_layout_loc` it_layout it →
-  val_to_Z_weak vo it = Some z1 →
-  val_to_Z_weak ve it = Some z2 →
+  val_to_Z vo it = Some z1 →
+  val_to_Z ve it = Some z2 →
   length vd = bytes_per_int it →
   (bytes_per_int it ≤ bytes_per_addr)%nat →
   z1 ≠ z2 →
@@ -268,7 +268,7 @@ Proof.
   iIntros (σ1) "((%&Hhctx&?)&Hfctx)".
   iDestruct (heap_mapsto_has_alloc_id with "Hl1") as %Haid1.
   iDestruct (heap_mapsto_has_alloc_id with "Hl2") as %Haid2.
-  move: (Hvo) (Hve) => /val_to_Z_weak_length ? /val_to_Z_weak_length ?.
+  move: (Hvo) (Hve) => /val_to_Z_length ? /val_to_Z_length ?.
   iDestruct (heap_mapsto_lookup_q (λ st : lock_state, ∃ n : nat, st = RSt n) with "Hhctx Hl1") as %? => //. { naive_solver. }
   iDestruct (heap_mapsto_lookup_1 (λ st : lock_state, st = RSt 0%nat) with "Hhctx Hl2") as %? => //.
   iModIntro. iSplit; first by eauto 15 using CasFailS.
@@ -286,8 +286,8 @@ Lemma wp_cas_suc vl1 vl2 vd vo ve z1 z2 Φ l1 l2 it E q:
   val_to_loc vl2 = Some l2 →
   l1 `has_layout_loc` it_layout it →
   l2 `has_layout_loc` it_layout it →
-  val_to_Z_weak vo it = Some z1 →
-  val_to_Z_weak ve it = Some z2 →
+  val_to_Z vo it = Some z1 →
+  val_to_Z ve it = Some z2 →
   length vd = bytes_per_int it →
   (bytes_per_int it ≤ bytes_per_addr)%nat →
   z1 = z2 →
@@ -299,7 +299,7 @@ Proof.
   iIntros (σ1) "((%&Hhctx&?)&Hfctx)".
   iDestruct (heap_mapsto_has_alloc_id with "Hl1") as %Haid1.
   iDestruct (heap_mapsto_has_alloc_id with "Hl2") as %Haid2.
-  move: (Hvo) (Hve) => /val_to_Z_weak_length ? /val_to_Z_weak_length ?.
+  move: (Hvo) (Hve) => /val_to_Z_length ? /val_to_Z_length ?.
   iDestruct (heap_mapsto_lookup_1 (λ st : lock_state, st = RSt 0%nat) with "Hhctx Hl1") as %? => //.
   iDestruct (heap_mapsto_lookup_q (λ st : lock_state, ∃ n : nat, st = RSt n) with "Hhctx Hl2") as %? => //. { naive_solver. }
   iModIntro. iSplit; first by eauto 15 using CasSucS.
@@ -313,8 +313,8 @@ Proof.
 Qed.
 
 Lemma wp_neg_int Φ v v' n E it:
-  val_to_Z_weak v it = Some n →
-  val_of_Z (-n) it = Some v' →
+  val_to_Z v it = Some n →
+  val_of_Z (-n) it None = Some v' →
   ▷ Φ (v') -∗ WP UnOp NegOp (IntOp it) (Val v) @ E {{ Φ }}.
 Proof.
   iIntros (Hv Hv') "HΦ".
@@ -325,8 +325,8 @@ Proof.
 Qed.
 
 Lemma wp_cast_int Φ v v' i E its itt:
-  val_to_int_repr v its = Some i →
-  val_of_int_repr i itt = Some v' →
+  val_to_Z v its = Some i →
+  val_of_Z i itt (val_to_byte_prov v) = Some v' →
   ▷ Φ (v') -∗ WP UnOp (CastOp (IntOp itt)) (IntOp its) (Val v) @ E {{ Φ }}.
 Proof.
   iIntros (Hv Hv') "HΦ".
@@ -347,22 +347,23 @@ Proof.
   - move => ->. by econstructor.
 Qed.
 
-Lemma wp_cast_ptr_int Φ v v' l E it:
+Lemma wp_cast_ptr_int Φ v v' l E it p:
   val_to_loc v = Some l →
-  val_of_int_repr (IRLoc l) it = Some v' →
+  l.1 = ProvAlloc p →
+  val_of_Z l.2 it p = Some v' →
   alloc_alive_loc l ∧ ▷ Φ (v') -∗
   WP UnOp (CastOp (IntOp it)) PtrOp (Val v) @ E {{ Φ }}.
 Proof.
-  iIntros (Hv Hv') "HΦ".
+  iIntros (Hv Hp Hv') "HΦ".
   iApply wp_unop_det. iSplit; [iDestruct "HΦ" as "[HΦ _]" | iDestruct "HΦ" as "[_ $]"].
   iIntros (σ ?) "Hctx". iDestruct (alloc_alive_loc_to_block_alive with "HΦ Hctx") as %Hb.
   iPureIntro. split.
-  - move: (Hb) => [?[??]]. have ? := val_to_of_loc NULL_loc. inversion 1; unfold NULL in *; by simplify_eq.
+  - have ? := val_to_of_loc NULL_loc. inversion 1; unfold NULL in *; destruct l; by simplify_eq/=.
   - move => ->. by econstructor.
 Qed.
 
 Lemma wp_cast_null_int Φ v E it:
-  val_of_Z 0 it = Some v →
+  val_of_Z 0 it None = Some v →
   ▷ Φ v -∗
   WP UnOp (CastOp (IntOp it)) PtrOp (Val NULL) @ E {{ Φ }}.
 Proof.
@@ -374,39 +375,42 @@ Proof.
   - move => ->. by econstructor.
 Qed.
 
-Lemma wp_cast_int_ptr_weak Φ v l E it:
-  val_to_loc_weak v it = Some l →
-  (∀ i, ▷ Φ (val_of_loc (i, l.2))) -∗
+Lemma wp_cast_int_ptr_weak Φ v a E it:
+  val_to_Z v it = Some a →
+  (∀ i, ▷ Φ (val_of_loc (i, a))) -∗
   WP UnOp (CastOp PtrOp) (IntOp it) (Val v) @ E {{ Φ }}.
 Proof.
   iIntros (Hv) "HΦ".
   iApply wp_unop.
   iIntros (σ) "Hctx". iSplit; [iPureIntro; eexists _; by econstructor |].
   iIntros "!>" (v' Hv'). iFrame.
-  inversion Hv'; simplify_eq. destruct l; simplify_eq/=; case_bool_decide; [ iApply "HΦ"|].
+  inversion Hv'; simplify_eq.
+  case_bool_decide; [ iApply "HΦ"|].
   case_bool_decide; simplify_eq; iApply "HΦ".
 Qed.
 
-Lemma wp_cast_int_ptr_alive Φ v l E it:
-  val_to_loc_weak v it = Some l →
+Lemma wp_cast_int_ptr_alive Φ v a p l E it:
+  val_to_Z v it = Some a →
+  val_to_byte_prov v = Some p →
+  l = (ProvAlloc (Some p), a) →
   loc_in_bounds l 0 -∗
   alloc_alive_loc l ∧ ▷ Φ (val_of_loc l) -∗
   WP UnOp (CastOp PtrOp) (IntOp it) (Val v) @ E {{ Φ }}.
 Proof.
-  iIntros (Hv) "#Hlib HΦ".
+  iIntros (Hv Hp ->) "#Hlib HΦ".
   iApply wp_unop_det. iSplit; [iDestruct "HΦ" as "[HΦ _]" | iDestruct "HΦ" as "[_ $]"].
   iIntros (σ ?) "Hctx".
-  iAssert ⌜valid_ptr l σ.(st_heap)⌝%I as %?. {
+  iAssert ⌜valid_ptr (ProvAlloc (Some p), a) σ.(st_heap)⌝%I as %?. {
     iSplit; [ |iApply (loc_in_bounds_to_heap_loc_in_bounds with "Hlib Hctx")].
     by iApply (alloc_alive_loc_to_block_alive with "[HΦ] Hctx").
   }
   iPureIntro. split.
-  - by inversion 1; simplify_eq; case_bool_decide.
-  - move => ->. econstructor; [done..|]. by case_bool_decide.
+  - inversion 1; simplify_eq; case_bool_decide; by rewrite ->Hp in *.
+  - move => ->. econstructor; [done..|]. rewrite Hp. by case_bool_decide.
 Qed.
 
 Lemma wp_copy_alloc_id Φ it a l v1 v2 E:
-  val_to_Z_weak v1 it = Some a →
+  val_to_Z v1 it = Some a →
   val_to_loc v2 = Some l →
   loc_in_bounds (l.1, a) 0 -∗
   alloc_alive_loc l ∧ ▷ Φ (val_of_loc (l.1, a)) -∗
@@ -425,9 +429,10 @@ Proof.
   by iApply wp_value.
 Qed.
 
-Lemma wp_ptr_relop Φ op v1 v2 l1 l2 E b:
+Lemma wp_ptr_relop Φ op v1 v2 v l1 l2 E b:
   val_to_loc v1 = Some l1 →
   val_to_loc v2 = Some l2 →
+  val_of_Z (Z_of_bool b) i32 None = Some v →
   match op with
   | EqOp => Some (bool_decide (l1.2 = l2.2))
   | NeOp => Some (bool_decide (l1.2 ≠ l2.2))
@@ -438,10 +443,10 @@ Lemma wp_ptr_relop Φ op v1 v2 l1 l2 E b:
   | _ => None
   end = Some b →
   loc_in_bounds l1 0 -∗ loc_in_bounds l2 0 -∗
-  (alloc_alive_loc l1 ∧ alloc_alive_loc l2 ∧ ▷ Φ (i2v (Z_of_bool b) i32)) -∗
+  (alloc_alive_loc l1 ∧ alloc_alive_loc l2 ∧ ▷ Φ v) -∗
   WP BinOp op PtrOp PtrOp (Val v1) (Val v2) @ E {{ Φ }}.
 Proof.
-  iIntros (Hv1 Hv2 Hop) "#Hl1 #Hl2 HΦ".
+  iIntros (Hv1 Hv2 Hv Hop) "#Hl1 #Hl2 HΦ".
   iDestruct (loc_in_bounds_has_alloc_id with "Hl1") as %[??].
   iDestruct (loc_in_bounds_has_alloc_id with "Hl2") as %[??].
   iApply wp_binop. iIntros (σ) "Hσ".
@@ -462,7 +467,7 @@ Qed.
 
 Lemma wp_ptr_offset Φ vl l E it o ly vo:
   val_to_loc vl = Some l →
-  val_to_Z_weak vo it = Some o →
+  val_to_Z vo it = Some o →
   loc_in_bounds (l offset{ly}ₗ o) 0 -∗
   ▷ Φ (val_of_loc (l offset{ly}ₗ o)) -∗
   WP Val vl at_offset{ ly , PtrOp, IntOp it} Val vo @ E {{ Φ }}.
@@ -478,7 +483,7 @@ Qed.
 
 Lemma wp_ptr_neg_offset Φ vl l E it o ly vo:
   val_to_loc vl = Some l →
-  val_to_Z_weak vo it = Some o →
+  val_to_Z vo it = Some o →
   loc_in_bounds (l offset{ly}ₗ -o) 0 -∗
   ▷ Φ (val_of_loc (l offset{ly}ₗ -o)) -∗
   WP Val vl at_neg_offset{ ly , PtrOp, IntOp it} Val vo @ E {{ Φ }}.
@@ -501,11 +506,11 @@ Lemma wp_get_member Φ vl l sl n E:
 Proof.
   iIntros (Hvl [i Hi]) "#Hl HΦ".
   rewrite /GetMember/GetMemberLoc/offset_of Hi /=.
-  have [|v Hv]:= (val_of_Z_is_Some size_t (offset_of_idx sl.(sl_members) i)). {
+  have [|v Hv]:= (val_of_Z_is_Some None size_t (offset_of_idx sl.(sl_members) i)). {
     split; first by rewrite /min_int/=; lia. by apply offset_of_bound.
   }
   rewrite Hv /=. move: Hv => /val_to_of_Z Hv.
-  iApply wp_ptr_offset; [done| by apply: val_to_Z_to_int_repr_Z | | ].
+  iApply wp_ptr_offset; [done| done | | ].
   { have ? := offset_of_idx_le_size sl i. rewrite offset_loc_sz1 //.
     iApply (loc_in_bounds_offset with "Hl"); simpl; [done| destruct l => /=; lia  | destruct l => /=; lia ]. }
   by rewrite offset_loc_sz1.
@@ -521,11 +526,11 @@ Qed.
 
 Lemma wp_offset_of Φ s m i E:
   offset_of s.(sl_members) m = Some i →
-  (∀ v, ⌜val_of_Z i size_t = Some v⌝ -∗ Φ v) -∗
+  (∀ v, ⌜val_of_Z i size_t None = Some v⌝ -∗ Φ v) -∗
   WP OffsetOf s m @ E {{ Φ }}.
 Proof.
   rewrite /OffsetOf. iIntros (Ho) "HΦ".
-  have [|? Hs]:= (val_of_Z_is_Some size_t i). {
+  have [|? Hs]:= (val_of_Z_is_Some None size_t i). {
     split; first by rewrite /min_int/=; lia.
     move: Ho => /fmap_Some[?[?->]].
     by apply offset_of_bound.
@@ -539,7 +544,7 @@ Lemma wp_offset_of_union Φ ul m E:
 Proof. by iApply @wp_value. Qed.
 
 Lemma wp_if Φ it v e1 e2 n:
-  val_to_Z_weak v it = Some n →
+  val_to_Z v it = Some n →
   (if decide (n = 0) then WP coerce_rtexpr e2 {{ Φ }} else WP coerce_rtexpr e1 {{ Φ }}) -∗
   WP IfE (IntOp it) (Val v) e1 e2 {{ Φ }}.
 Proof.
@@ -837,7 +842,7 @@ Proof.
 Qed.
 
 Lemma wps_switch Q Ψ v n ss def m it:
-  val_to_Z_weak v it = Some n →
+  val_to_Z v it = Some n →
   (∀ i, m !! n = Some i → is_Some (ss !! i)) →
   WPs default def (i ← m !! n; ss !! i) {{ Q, Ψ }} -∗ WPs (Switch it (Val v) m ss def) {{ Q , Ψ }}.
 Proof.
@@ -850,7 +855,7 @@ Qed.
 
 (** a version of wps_switch which is directed by ss instead of n *)
 Lemma wps_switch' Q Ψ v n ss def m it:
-  val_to_Z_weak v it = Some n →
+  val_to_Z v it = Some n →
   map_Forall (λ _ i, is_Some (ss !! i)) m →
   ([∧ list] i↦s∈ss, ⌜m !! n = Some i⌝ -∗ WPs s {{ Q, Ψ }}) ∧
   (⌜m !! n = None⌝ -∗ WPs def {{ Q, Ψ }}) -∗
@@ -865,7 +870,7 @@ Proof.
 Qed.
 
 Lemma wps_if Q Ψ v s1 s2 n:
-  val_to_Z_weak v bool_it = Some n →
+  val_to_Z v bool_it = Some n →
   (if decide (n = 0) then WPs s2 {{ Q, Ψ }} else WPs s1 {{ Q, Ψ }}) -∗
   WPs (if: (Val v) then s1 else s2) {{ Q , Ψ }}.
 Proof.
@@ -875,7 +880,7 @@ Proof.
 Qed.
 
 Lemma wps_assert Q Ψ v s n:
-  val_to_Z_weak v bool_it = Some n → n ≠ 0 →
+  val_to_Z v bool_it = Some n → n ≠ 0 →
   WPs s {{ Q, Ψ }} -∗
   WPs (assert: Val v; s) {{ Q , Ψ }}.
 Proof.
