theories/typing/padded.v
@@ -196,7 +196,7 @@ Section padded.
       typed_bin_op v2 (v2 ◁ᵥ n @ int it) p (p ◁ₗ{β} padded ty lyty ly) (PtrOffsetOp u8) (IntOp it) PtrOp T.
   Proof.
     iIntros "HT" (Hint) "Hp". iIntros (Φ) "HΦ".
-    move: (Hint) => /val_to_Z_weak_in_range?.
+    move: (Hint) => /val_to_Z_in_range?.
     iDestruct ("HT" with "[//]") as (???) "HT".
     iDestruct (split_padded (Z.to_nat n) with "Hp") as "[H1 H2]"; [lia..|].
     rewrite -!(offset_loc_sz1 u8)// Z2Nat.id; [|lia].
